Introduce separate types for SmtBool and SmtArith.

ConcreteToSymbolicLemmas.v
@@ -8,16 +8,16 @@ Require Import Coq.Strings.String.
 Local Open Scope string_scope.
 
 (* Apply SmtValuation f to every entry in the symbolic state across all 3 maps *)
-Definition eval_sym_state (s: ProgramState SmtExpr) (f : SmtValuation) : ProgramState uint8 :=
-  {| header_map := fun h => eval_smt_expr (header_map SmtExpr s h) f;
-     ctrl_plane_map := fun c => eval_smt_expr (ctrl_plane_map SmtExpr s c) f;
-     state_var_map := fun sv => eval_smt_expr (state_var_map SmtExpr s sv) f |}.
+Definition eval_sym_state (s: ProgramState SmtArithExpr) (f : SmtValuation) : ProgramState uint8 :=
+  {| header_map := fun h => eval_smt_arith (header_map SmtArithExpr s h) f;
+     ctrl_plane_map := fun c => eval_smt_arith (ctrl_plane_map SmtArithExpr s c) f;
+     state_var_map := fun sv => eval_smt_arith (state_var_map SmtArithExpr s sv) f |}.
 
 (* Simpler lemma with no state update *)
 Lemma commute_smt_conc_expr:
-  forall (ho: HdrOp) (s : ProgramState SmtExpr) (f : SmtValuation),
+  forall (ho: HdrOp) (s : ProgramState SmtArithExpr) (f : SmtValuation),
     eval_hdr_op_expr_uint8 ho (eval_sym_state s f) =
-    eval_smt_expr (eval_hdr_op_expr_smt ho s) f.
+    eval_smt_arith (eval_hdr_op_expr_smt ho s) f.
 Proof.
   intros ho s f.
   destruct ho, f0, arg1, arg2; simpl; try reflexivity.
@@ -28,9 +28,9 @@ Axiom functional_extensionality :
     (forall x, f x = g x) -> f = g.
 
 Lemma commute_update_eval:
-  forall (s : ProgramState SmtExpr) (f : SmtValuation) (sv : StateVar) (v : SmtExpr),
+  forall (s : ProgramState SmtArithExpr) (f : SmtValuation) (sv : StateVar) (v : SmtArithExpr),
     eval_sym_state (update_state s sv v) f =
-    update_state (eval_sym_state s f) sv (eval_smt_expr v f).
+    update_state (eval_sym_state s f) sv (eval_smt_arith v f).
 Proof.
   intros s f sv v.
   destruct s as [con_ctrl con_hdr con_state].
@@ -49,9 +49,9 @@ Proof.
 Qed.
 
 Lemma commute2_update_eval:
-  forall (s : ProgramState SmtExpr) (f : SmtValuation) (h : Header) (v : SmtExpr),
+  forall (s : ProgramState SmtArithExpr) (f : SmtValuation) (h : Header) (v : SmtArithExpr),
     eval_sym_state (update_hdr s h v) f =
-    update_hdr (eval_sym_state s f) h (eval_smt_expr v f).
+    update_hdr (eval_sym_state s f) h (eval_smt_arith v f).
 Proof.
   intros s f h v.
   destruct s as [con_ctrl con_hdr con_state].
@@ -73,7 +73,7 @@ Qed.
   concretizing and then evaluating EQUALS
   evaluating and then concretizing *)
 Lemma commute_sym_conc:
-  forall (ho : HdrOp) (s : ProgramState SmtExpr) (f : SmtValuation),
+  forall (ho : HdrOp) (s : ProgramState SmtArithExpr) (f : SmtValuation),
      eval_hdr_op_assign_uint8 ho (eval_sym_state s f) =
       eval_sym_state (eval_hdr_op_assign_smt ho s) f.
 Proof.
@@ -88,8 +88,8 @@ Qed.
 (* Joe's theorem relating the concrete and symbolic worlds translated into rocq slack *)
 Lemma symbolic_vs_concrete :
   forall (f : SmtValuation) (ho : HdrOp)
-         (c1 : ProgramState uint8) (s1 : ProgramState SmtExpr)
-         (c2 : ProgramState uint8) (s2 : ProgramState SmtExpr),
+         (c1 : ProgramState uint8) (s1 : ProgramState SmtArithExpr)
+         (c2 : ProgramState uint8) (s2 : ProgramState SmtArithExpr),
     c1 = eval_sym_state s1 f ->
     c2 = eval_hdr_op_assign ho c1 ->
     s2 = eval_hdr_op_assign ho s1 ->
